Progress on model_E1E2_L6 adequacy theorem.
Several changes have been made:

- Introduce lemmas for refine_E1E2_LX and interpreters.
- Mocked out model_E1E2_LX_sound lemmas
- model_E1E2_LX_sound are QEDd for each LX > L0
  + depends on some SERIOUS admitted lemmas, though.
- Had to expose type of SBytes... Ended up breaking a few proofs as
  more stuff would unfold.
- Had to expose provenance types.
- Added conversions between memories in different languages.
- Needed InfFin and FinInf versions of some refine_OOM_h lemmas.
- Had to patch up extraction again.

src/coq/Handlers/MemoryModules/FiniteAddresses.v
@@ -78,7 +78,13 @@ End FinPTOI.
 Module FinPROV : PROVENANCE(FinAddr)
 with Definition Prov := Prov
 with Definition address_provenance
-    := fun (a : FinAddr.addr) => snd a.
+    := fun (a : FinAddr.addr) => snd a
+with Definition Provenance := Provenance
+with Definition AllocationId := AllocationId
+with Definition wildcard_prov := wildcard_prov
+with Definition nil_prov := nil_prov
+with Definition initial_provenance := 0%N.
+
   Definition Provenance := Provenance.
   Definition AllocationId := AllocationId.
   Definition Prov := Prov.
@@ -273,7 +279,13 @@ with Definition address_provenance
   Definition show_allocation_id (aid : AllocationId) := Show.show aid.
 End FinPROV.
 
-Module FinITOP : ITOP(FinAddr)(FinPROV)(FinPTOI).
+Module FinITOP : ITOP(FinAddr)(FinPROV)(FinPTOI)
+with Definition int_to_ptr :=
+  fun (i : Z) (pr : Prov) =>
+    if (i <? 0)%Z || (i >=? Int64.modulus)%Z
+    then Oom ("FinITOP.int_to_ptr: out of range (" ++ show i ++ ").")
+    else NoOom (Int64.repr i, pr).
+
   Import FinAddr.
   Import FinPROV.
   Import FinPTOI.
