src/coq/Semantics/LLVMParams.v
@@ -23,7 +23,13 @@ Module Type LLVMParamsBig <: LLVMParams.
   Declare Module I2P_BIG : ITOP_BIG ADDR PROV PTOI ITOP.
 End LLVMParamsBig.
 
-Module Make (ADDR' : ADDRESS) (IP' : INTPTR) (SIZEOF' : Sizeof) (PTOI' : PTOI ADDR') (PROV' : PROVENANCE ADDR') (ITOP' : ITOP ADDR' PROV' PTOI') : LLVMParams with Module ADDR := ADDR'.
+Module Make (ADDR' : ADDRESS) (IP' : INTPTR) (SIZEOF' : Sizeof) (PTOI' : PTOI ADDR') (PROV' : PROVENANCE ADDR') (ITOP' : ITOP ADDR' PROV' PTOI') : LLVMParams
+with Module ADDR := ADDR'
+with Module IP := IP'
+with Module SIZEOF := SIZEOF'
+with Module PTOI := PTOI'
+with Module PROV := PROV'
+with Module ITOP := ITOP'.
   Module ADDR := ADDR'.
   Module IP := IP'.
   Module SIZEOF := SIZEOF'.
@@ -33,7 +39,15 @@ Module Make (ADDR' : ADDRESS) (IP' : INTPTR) (SIZEOF' : Sizeof) (PTOI' : PTOI AD
   Module Events := LLVMEvents.Make ADDR IP SIZEOF.
 End Make.
 
-Module MakeBig (ADDR' : ADDRESS) (IP' : INTPTR) (SIZEOF' : Sizeof) (PTOI' : PTOI ADDR') (PROV' : PROVENANCE ADDR') (ITOP' : ITOP ADDR' PROV' PTOI') (IP_BIG' : INTPTR_BIG IP') (I2P_BIG' : ITOP_BIG ADDR' PROV' PTOI' ITOP') : LLVMParamsBig with Module ADDR := ADDR'.
+Module MakeBig (ADDR' : ADDRESS) (IP' : INTPTR) (SIZEOF' : Sizeof) (PTOI' : PTOI ADDR') (PROV' : PROVENANCE ADDR') (ITOP' : ITOP ADDR' PROV' PTOI') (IP_BIG' : INTPTR_BIG IP') (I2P_BIG' : ITOP_BIG ADDR' PROV' PTOI' ITOP') : LLVMParamsBig
+with Module ADDR := ADDR'
+with Module IP := IP'
+with Module SIZEOF := SIZEOF'
+with Module PTOI := PTOI'
+with Module PROV := PROV'
+with Module ITOP := ITOP'
+with Module IP_BIG := IP_BIG'
+with Module I2P_BIG := I2P_BIG'.
   Module ADDR := ADDR'.
   Module IP := IP'.
   Module SIZEOF := SIZEOF'.
